theories/typing/lib/rc/rc.v
@@ -60,16 +60,16 @@ Section rc.
     (∃ st : rc_stR, own γ (● st) ∗
       match st with
       | (Some (Cinl (q, strong)), weak) => ∃ q',
-        l ↦ #(Zpos strong) ∗ shift_loc l 1 ↦ #(S weak) ∗ † l…(2 + ty.(ty_size)) ∗
+        l ↦ #(Zpos strong) ∗ (l +ₗ 1) ↦ #(S weak) ∗ † l…(2 + ty.(ty_size)) ∗
           ⌜(q + q')%Qp = 1%Qp⌝ ∗ q'.[ν] ∗
           (* We keep this view shift decomposed because we store the persistent
              part in ty_own, to make it available with one step less. *)
-          ([†ν] ={↑lftN}=∗ ▷ shift_loc l 2 ↦∗: ty.(ty_own) tid)
+          ([†ν] ={↑lftN}=∗ ▷ (l +ₗ 2) ↦∗: ty.(ty_own) tid)
       | (Some (Cinr _), weak) =>
-        l ↦ #0 ∗ shift_loc l 1 ↦ #(S weak)
+        l ↦ #0 ∗ (l +ₗ 1) ↦ #(S weak)
       | (None, (S _) as weak) =>
-        l ↦ #0 ∗ shift_loc l 1 ↦ #weak ∗ † l…(2 + ty.(ty_size)) ∗
-          shift_loc l 2 ↦∗: λ vl, ⌜length vl = ty.(ty_size)⌝
+        l ↦ #0 ∗ (l +ₗ 1) ↦ #weak ∗ † l…(2 + ty.(ty_size)) ∗
+          (l +ₗ 2) ↦∗: λ vl, ⌜length vl = ty.(ty_size)⌝
       | _ => True
       end)%I.
 
@@ -85,7 +85,7 @@ Section rc.
               (* We use this disjunction, and not simply [ty_shr] here,
                  because [weak_new] cannot prove ty_shr, even for a dead
                  lifetime. *)
-              (ty.(ty_shr) ν tid (shift_loc l 2) ∨ [†ν]) ∗
+              (ty.(ty_shr) ν tid (l +ₗ 2) ∨ [†ν]) ∗
               □ (1.[ν] ={↑lftN,∅}▷=∗ [†ν]))%I.
 
   Global Instance rc_persist_ne ν γ l n :
@@ -114,8 +114,8 @@ Section rc.
               shared protocol or the full ownership of the
               content. The reason is that get_mut does not have the
               masks to rebuild the invariants. *)
-           (l ↦ #1 ∗ shift_loc l 1 ↦ #1 ∗ † l…(2 + ty.(ty_size)) ∗
-            ▷ shift_loc l 2 ↦∗: ty.(ty_own) tid) ∨
+           (l ↦ #1 ∗ (l +ₗ 1) ↦ #1 ∗ † l…(2 + ty.(ty_size)) ∗
+            ▷ (l +ₗ 2) ↦∗: ty.(ty_own) tid) ∨
            (∃ γ ν q, rc_persist tid ν γ l ty ∗ own γ (rc_tok q) ∗ q.[ν])
          | _ => False end;
        ty_shr κ tid l :=
@@ -241,25 +241,25 @@ Section code.
     !#l
     {{{ strong, RET #(Zpos strong); l ↦ #(Zpos strong) ∗
         (((⌜strong = 1%positive⌝ ∗
-           (∃ weak : Z, shift_loc l 1 ↦ #weak ∗
+           (∃ weak : Z, (l +ₗ 1) ↦ #weak ∗
              ((⌜weak = 1⌝ ∗
                |={⊤,∅}▷=> † l…(2 + ty.(ty_size)) ∗
-                          ▷ shift_loc l 2 ↦∗: ty.(ty_own) tid ∗ na_own tid F) ∨
+                          ▷ (l +ₗ 2) ↦∗: ty.(ty_own) tid ∗ na_own tid F) ∨
              (⌜weak > 1⌝ ∗
-              ((l ↦ #1 -∗ shift_loc l 1 ↦ #weak
+              ((l ↦ #1 -∗ (l +ₗ 1) ↦ #weak
                 ={⊤}=∗ na_own tid F ∗ ty_own (rc ty) tid [ #l ]) ∧
-               (l ↦ #0 -∗ shift_loc l 1 ↦ #(weak - 1)
-                ={⊤,∅}▷=∗ ▷ shift_loc l 2 ↦∗: ty.(ty_own) tid ∗
-                (shift_loc l 2 ↦∗: (λ vl, ⌜length vl = ty.(ty_size)⌝)
+               (l ↦ #0 -∗ (l +ₗ 1) ↦ #(weak - 1)
+                ={⊤,∅}▷=∗ ▷ (l +ₗ 2) ↦∗: ty.(ty_own) tid ∗
+                ((l +ₗ 2) ↦∗: (λ vl, ⌜length vl = ty.(ty_size)⌝)
                  ={⊤}=∗ na_own tid F)))))) ∧
            (l ↦ #0 ={⊤,∅}▷=∗
-             ▷ shift_loc l 2 ↦∗: ty.(ty_own) tid ∗ † l…(2 + ty.(ty_size)) ∗ na_own tid F ∗
+             ▷ (l +ₗ 2) ↦∗: ty.(ty_own) tid ∗ † l…(2 + ty.(ty_size)) ∗ na_own tid F ∗
              (na_own tid F ={⊤}=∗ ∃ weak : Z,
-                shift_loc l 1 ↦ #weak ∗
+                (l +ₗ 1) ↦ #weak ∗
                 ((⌜weak = 1⌝ ∗ l ↦ #0 ∗ na_own tid F) ∨
                  (⌜weak > 1⌝ ∗
-                   († l…(2 + ty.(ty_size)) -∗ shift_loc l 1 ↦ #(weak-1) -∗
-                    shift_loc l 2 ↦∗: (λ vl, ⌜length vl = ty.(ty_size)⌝)
+                   († l…(2 + ty.(ty_size)) -∗ (l +ₗ 1) ↦ #(weak-1) -∗
+                    (l +ₗ 2) ↦∗: (λ vl, ⌜length vl = ty.(ty_size)⌝)
                     ={⊤}=∗ na_own tid F))))))
          ) ∨
          (⌜(1 < strong)%positive⌝ ∗
@@ -1035,13 +1035,13 @@ Section code.
         iDestruct (ty_size_eq with "Hty") as %?.
         wp_apply (wp_memcpy with "[$Hlr3 $H↦vlr]"); [lia..|]. iIntros "[Hlr3 Hvlr]".
         wp_seq. wp_write. wp_op. iMod ("Hproto" with "[Hvlr]") as "Hna"; first by eauto.
-        iMod ("Hclose2" $! (shift_loc lr 2 ↦∗: ty_own ty tid)%I
+        iMod ("Hclose2" $! ((lr +ₗ 2) ↦∗: ty_own ty tid)%I
               with "[Hrc' Hlr1 Hlr2 H†] [Hlr3 Hty]") as "[Hb Hα1]".
         { iIntros "!> H !>". iExists [_]. rewrite heap_mapsto_vec_singleton. iFrame.
           iLeft. iFrame. rewrite Z2Nat.inj_pos Pos2Nat.inj_succ SuccNat2Pos.id_succ //. }
         { iExists _. iFrame. }
         iMod ("Hclose1" with "[$Hα1 $Hα2] HL") as "HL".
-        iApply (type_type _ _ _ [ r ◁ box (uninit 1); #(shift_loc lr 2) ◁ &uniq{α} ty;
+        iApply (type_type _ _ _ [ r ◁ box (uninit 1); #(lr +ₗ 2) ◁ &uniq{α} ty;
                                   rcx ◁ box (uninit 1)]
                 with "[] LFT HE Hna HL Hk [-]"); last first.
         { rewrite 2!tctx_interp_cons tctx_interp_singleton !tctx_hasty_val
@@ -1092,7 +1092,7 @@ Section code.
       wp_apply (wp_delete with "[$Hcl↦ Hcl†]");
         [lia|by replace (length vl) with (ty.(ty_size))|].
       iIntros "_". wp_seq. wp_write.
-      iMod ("Hclose2" $! (shift_loc l' 2 ↦∗: ty_own ty tid)%I with
+      iMod ("Hclose2" $! ((l' +ₗ 2) ↦∗: ty_own ty tid)%I with
           "[Hrc' Hl' Hl'1  Hl'†] [Hl'2 Hown]") as "[Hl' Hα1]".
       { iIntros "!> H". iExists [_]. rewrite heap_mapsto_vec_singleton. iFrame.
         iLeft. iFrame. iDestruct "Hl'†" as "[?|%]"=>//.
