theories/typing/lib/rwlock/rwlock_code.v
@@ -97,7 +97,7 @@ Section rwlock_functions.
     rewrite tctx_interp_cons tctx_interp_singleton !tctx_hasty_val.
     iDestruct "HT" as "[Hx Hx']". destruct x' as [[|lx'|]|];  try iDestruct "Hx'" as "[]".
     iAssert (&{α} (∃ (z : Z), lx' ↦ #z ∗ ⌜-1 ≤ z⌝) ∗
-        (&uniq{α} ty).(ty_own) tid [ #(shift_loc lx' 1)])%I with "[> Hx']" as "[_ Hx']".
+        (&uniq{α} ty).(ty_own) tid [ #(lx' +ₗ 1)])%I with "[> Hx']" as "[_ Hx']".
     { iApply bor_sep; [done..|]. iApply (bor_proper with "Hx'"). iSplit.
       - iIntros "[H1 H2]". iDestruct "H1" as (z) "[??]". iDestruct "H2" as (vl) "[??]".
         iExists (_::_). rewrite heap_mapsto_vec_cons. iFrame. iFrame.
@@ -108,7 +108,7 @@ Section rwlock_functions.
     destruct x as [[|lx|]|]; try done. iDestruct "Hx" as "[Hx Hx†]".
     iDestruct "Hx" as (vl) "[Hx↦ Hx]". rewrite uninit_own. wp_op.
     iApply (type_type _ _ _
-            [ #lx ◁ box (uninit 1); #(shift_loc lx' 1) ◁ &uniq{α}ty]
+            [ #lx ◁ box (uninit 1); #(lx' +ₗ 1) ◁ &uniq{α}ty]
             with "[] LFT HE Hna HL HC [-]"); last first.
     { rewrite tctx_interp_cons tctx_interp_singleton !tctx_hasty_val' //. iFrame.
       iNext. iExists _. rewrite uninit_own. iFrame. }
@@ -181,7 +181,7 @@ Section rwlock_functions.
       destruct (decide (Z_of_rwlock_st st = Z_of_rwlock_st st')) as [->|?]=>?.
       + iApply (wp_cas_int_suc with "Hlx"); first done. iNext. iIntros "Hlx".
         iAssert (∃ qν ν, (qβ / 2).[β] ∗ (qν).[ν] ∗
-                         ty_shr ty (β ⊓ ν) tid (shift_loc lx 1) ∗
+                         ty_shr ty (β ⊓ ν) tid (lx +ₗ 1) ∗
                          own γ (◯ reading_st qν ν) ∗ rwlock_inv tid lx γ β ty ∗
                          ((1).[ν] ={↑lftN,∅}▷=∗ [†ν]))%I
           with "[> Hlx Hownst Hst Hβtok2]"
